\section{Complex Numbers}

\subsection{Arithmetic Operations}

\begin{enumerate}
\item
  Find the values of
  \[
  (1 + 2i)^3, \qquad \frac{5}{-3 + 4i}, \qquad
  \Bigl(\frac{2 + i}{3 - 2i}\Bigr)^2, \qquad (1 + i)^n + (1 - i)^n
  \]
  For the first problem, we have \((1 + 2i)^3 = (-3 + 4i)(1 + 2i) = -11 - 2i\).
  For the second problem, we should multiple by the conjugate
  \(\bar{z} = -3 - 4i\).
  \[
  \frac{5}{-3 + 4i}\frac{-3 - 4i}{-3 - 4i} = \frac{-15 - 20i}{25} =
  \frac{-3}{5} - \frac{4}{5}i
  \]
  For the third problem, we should first multiple by \(\bar{z} = 3 + 2i\).
  \[
  \frac{2 + i}{3 - 2i}\frac{3 + 2i}{3 + 2i} = \frac{8 + i}{13}
  \]
  Now we need to just square the result.
  \[
  \frac{1}{169}(8 + i)^2 = \frac{63 + 16i}{169}
  \]
  For the last problem, we will need to find the polar form of the complex
  numbers.
  Let \(z_1 = 1 + i\) and \(z_2 = 1 - i\).
  Then the modulus of \(z_1 = \sqrt{2} = z_2\).
  Let \(\phi_1\) and \(\phi_2\) be the angles associated with \(z_1\) and
  \(z_2\), respectively.
  Then \(\phi_1 = \arctan(1) = \frac{\pi}{4}\) and
  \(\phi_2 = \arctan(-1) = \frac{-\pi}{4}\).
  Then \(z_1 = \sqrt{2}e^{\pi i/4}\) and \(z_2 = \sqrt{2}e^{-\pi i/4}\).
  \begin{align*}
    z_1^n + z_2^n
    & = 2^{n/2}\bigl[e^{n\pi i/4} + e^{-n\pi i/4}\bigr]\\
    & = 2^{n/2 + 1}\biggl[\frac{e^{n\pi i/4} + e^{-n\pi i/4}}{2}\biggr]\\
    & = 2^{n/2 + 1}\cos\Bigl(\frac{n\pi}{4}\Bigr)
  \end{align*}
\item
  If \(z = x + iy\) (\(x\) and \(y\) real), find the real and imaginary parts
  of
  \[
  z^4, \qquad \frac{1}{z}, \qquad \frac{z - 1}{z + 1}, \qquad \frac{1}{z^2}
  \]
  For \(z^4\), we can use the binomial theorem since
  \((a + b)^n = \sum_{k = 0}^n\binom{n}{k}a^nb^{n - k}\).
  Therefore,
  \[
  (x + iy)^4 = \binom{4}{0}(iy)^4 + \binom{4}{1}x(iy)^3 +
  \binom{4}{2}x^2(iy)^2 + \binom{4}{3}x^3(iy) + \binom{4}{4}x^4 =
  y^4 - 4xy^3i - 6x^2y^2 + 4x^3yi + x^4
  \]
  Then the real and imaginary parts are
  \begin{align*}
    u(x, y) & = x^4 + y^4 - 6x^2y^2\\
    v(x, y) & = 4x^3y - 4xy^3
  \end{align*}
  For second problem, we need to multiple by the conjugate \(\bar{z}\).
  \[
  \frac{1}{x + iy}\frac{x - iy}{x - iy} = \frac{x - iy}{x^2 + y^2}
  \]
  so the real and imaginary parts are
  \begin{align*}
    u(x, y) & = \frac{x}{x^2 + y^2}\\
    v(x, y) & = \frac{-y}{x^2 + y^2}
  \end{align*}
  For the third problem, we have \(\frac{x - 1 + iy}{x + 1 - iy}\).
  Then \(\bar{z} = x + 1 + iy\).
  \[
  \frac{x - 1 + iy}{x + 1 - iy}\frac{x + 1 + iy}{x + 1 + iy} =
  \frac{x^2 - 1 + 2xyi}{(x + 1)^2 + y^2}
  \]
  Then real and imaginary parts are
  \begin{align*}
    u(x, y) & = \frac{x^2 - 1}{(x + 1)^2 + y^2}\\
    v(x, y) & = \frac{2xy}{(x + 1)^2 + y^2}
  \end{align*}
  For the last problem, we have
  \[
  \frac{1}{z^2} = \frac{x^2 - y^2 - 2xyi}{x^4 + 2x^2y^2 + y^4}
  \]
  so the real and imaginary parts are
  \begin{align*}
    u(x, y) & = \frac{x^2 - y^2}{x^4 + 2x^2y^2 + y^4}\\
    v(x, y) & = \frac{-2xy}{x^4 + 2x^2y^2 + y^4}
  \end{align*}
\item
  Show that \(\bigl(\frac{-1\pm i\sqrt{3}}{2}\bigr)^3 = 1\) and
  \(\bigl(\frac{\pm 1\pm i\sqrt{3}}{2}\bigr)^6 = 1\).
  \par\smallskip
  Both problems will can be handled easily by converting to polar form.
  Let \(z_1 = \frac{-1\pm i\sqrt{3}}{2}\).
  Then \(\lvert z_1\rvert = 1\).
  Let \(\phi_+\) be the angle for the positive \(z_1\) and \(\phi_-\) for the
  negative.
  Then \(\phi_+ = \arctan(-\sqrt{3}) = \frac{2\pi}{3}\) and
  \(\phi_- = \arctan(\sqrt{3}) = \frac{4\pi}{3}\).
  We can write \(z_{1+} = e^{2i\pi/3}\) and \(z_{1-} = e^{4i\pi/3}\).
  \begin{align*}
    z_{1+}^3 & = e^{2i\pi}\\
             & = 1\\
    z_{1-}^3 & = e^{4i\pi}\\
             & = 1
  \end{align*}
  Therefore, \(z_1^3 = 1\).
  For the second problem, \(\phi_{ij} = \pm\frac{\pi}{3}\) and
  \(\pm\frac{2\pi}{3}\) for \(i, j = +, -\) and the \(\lvert z_2\rvert = 1\).
  When we raise \(z\) to the sixth poewr, the argument becomes \(\pm 2\pi\) and
  \(\pm 4\pi\).
  \[
  e^{\pm 2i\pi} = e^{\pm 4i\pi} = z^6 = 1
  \]
\end{enumerate}

\subsection{Square Roots}
\begin{enumerate}
\item
  Compute
  \[
  \sqrt{i}, \qquad \sqrt{-i}, \qquad \sqrt{1 + i}, \qquad
  \sqrt{\frac{1 - i\sqrt{3}}{2}}
  \]
  For \(\sqrt{i}\), we are looking for \(x\) and \(y\) such that
  \begin{align}
    \sqrt{i} & = x + iy\notag\\
    i & = x^2 - y^2 + 2xyi\notag\\
    x^2 - y^2 & = 0\label{ch1sec2prob1a}\\
    2xy & = 1\label{ch1sec2prob1a2}
  \end{align}
  From \cref{ch1sec2prob1a}, we see that \(x^2 = y^2\) or \(\pm x = \pm y\).
  Also, note that \(i\) is the upper half plane (UHP).
  That is, the angle is positive so \(x = y\) and \(2x^2 = 1\) from
  \cref{ch1sec2prob1a2}.
  Therefore, \(\sqrt{i} = \frac{1}{\sqrt{2}}(1 + i)\).
  We also could have done this problem using the polar form of \(z\).
  Let \(z = i\).
  Then \(z = e^{i\pi/2}\) so \(\sqrt{z} = e^{i\pi/4}\) which is exactly what we
  obtained.
  For \(\sqrt{-i}\), let \(z = -i\).
  Then \(z\) in polar form is \(z = e^{-i\pi/2}\) so
  \(\sqrt{z} = e^{-i\pi/4} = \frac{1}{\sqrt{2}}(1 - i)\).
  For \(\sqrt{1 + i}\), let \(z = 1 + i\).
  Then \(z = \sqrt{2}e^{i\pi/4}\) so \(\sqrt{z} = 2^{1/4}e^{i\pi/8}\).
  Finally, for \(\sqrt{\frac{1 - i\sqrt{3}}{2}}\), let
  \(z = \frac{1 - i\sqrt{3}}{2}\).
  Then \(z = e^{-i\pi/3}\) so
  \(\sqrt{z} = e^{-i\pi/6} = \frac{1}{2}(\sqrt{3} - i)\).
\item
  Find the four values of \(\sqrt[4]{-1}\).
  \par\smallskip
  Let \(z = \sqrt[4]{-1}\) so \(z^4 = -1\).
  Let \(z = re^{i\theta}\) so \(r^4e^{4i\theta} = -1 = e^{i\pi(1 + 2k)}\).
    \begin{align*}
      r^4 & = 1\\
      \theta & = \frac{\pi}{4}(1 + 2k)
    \end{align*}
    where \(k = 0\), \(1\), \(2\), \(3\).
    Since when \(k = 4\), we have \(k = 0\).
    Then \(\theta = \frac{\pi}{4}\), \(\frac{3\pi}{4}\), \(\frac{5\pi}{4}\),
    and \(\frac{7\pi}{4}\).
    \[
    z = e^{i\pi/4}, e^{3i\pi/4}, e^{5i\pi/4}, e^{7i\pi/4}
    \]
\item
  Compute \(\sqrt[4]{i}\) and \(\sqrt[4]{-i}\).
  \par\smallskip
  Let \(z = \sqrt[4]{i}\) and \(z = re^{i\theta}\).
  Then \(r^4e^{4i\theta} = i = e^{i\pi/2}\).
    \begin{align*}
      r^4 & = 1\\
      \theta & = \frac{\pi}{8}
    \end{align*}
    so \(z = e^{i\pi/8}\).
    Now, let \(z = \sqrt[4]{-i}\).
    Then \(r^4e^{4i\theta} = e^{-i\pi/2}\) so \(z = e^{-i\pi/8}\).
\item
  Solve the quadratic equation
  \[
  z^2 + (\alpha + i\beta)z + \gamma + i\delta = 0.
  \]
  The quadratic equation is \(x = \frac{-b\pm\sqrt{b^2 - ac}}{2}\).
  For the complex polynomial, we have
  \[
  z = \frac{-\alpha - \beta i\pm
    \sqrt{\alpha^2 - \beta^2 - 4\gamma + i(2\alpha\beta - 4\delta)}}{2}
  \]
  Let
  \(a + bi = \sqrt{\alpha^2 - \beta^2 - 4\gamma + i(2\alpha\beta - 4\delta)}\).
  Then
  \[
  z = \frac{-\alpha - \beta\pm (a + bi)}{2}
  \]
\end{enumerate}

\subsection{Justification}

\begin{enumerate}
\item
  Show that the system of all matrices of the special form
  \[
  \begin{pmatrix}
    \alpha & \beta\\
    -\beta & \alpha
  \end{pmatrix},
  \]
  combined by matrix addition and matrix multiplication, is isomorphic to the
  field of complex numbers.
\item
  Show that the complex number system can be thought of as the field of all
  polynomials with real coefficients modulo the irreducible polynomial
  \(x^2 + 1\).
\end{enumerate}

\subsection{Conjugation, Absolute Value}
\begin{enumerate}
\item
  Verify by calculation the values of
  \[
  \frac{z}{z^2 + 1}
  \]
  for \(z = x + iy\) and \(\bar{z} = x - iy\) are conjugate.
  \par\smallskip
  For \(z\), we have that \(z^2 = x^2 - y^2 + 2xyi\).
  \begin{align*}
    \frac{z}{z^2 + 1}
    & = \frac{x + iy}{x^2 - y^2 + 1 + 2xyi}\\
    & = \frac{x + iy}{x^2 - y^2 + 1 + 2xyi}
      \frac{x^2 - y^2 + 1 - 2xyi}{x^2 - y^2 + 1 - 2xyi}\\
    & = \frac{x(x^2 - y^2 + 1) + 2xy^2 + iy(x^2 - y^2 + 1 - 2x^2)}
      {(x^2 - y^2 + 1)^2 + 4x^2y^2}\eqnumtag\label{1.4.1z}
  \end{align*}
  For \(\bar{z}\), we have that \(\bar{z}^2 = x^2 - y^2 - 2xyi\).
  \begin{align*}
    \frac{\bar{z}}{\bar{z}^2 + 1}
    & = \frac{x - iy}{x^2 - y^2 + 1 - 2xyi}\\
    & = \frac{x - iy}{x^2 - y^2 + 1 - 2xyi}
      \frac{x^2 - y^2 + 1 + 2xyi}{x^2 - y^2 + 1 + 2xyi}\\
    & = \frac{x(x^2 - y^2 + 1) + 2xy^2 - iy(x^2 - y^2 + 1 - 2x^2)}
      {(x^2 - y^2 + 1)^2 + 4x^2y^2}\eqnumtag\label{1.4.1barz}
  \end{align*}
  Therefore, we have that \cref{1.4.1z,1.4.1barz} are conjugates.
\item
  Find the absolute value (modulus) of
  \[
  -2i(3 + i)(2 + 4i)(1 + i)\qquad\text{and}\qquad
  \frac{(3 + 4i)(-1 + 2i)}{(-1 - i)(3 - i)}.
  \]
  When we expand the first problem, we have that
  \[
  z_1 = -2i(3 + i)(2 + 4i)(1 + i) = 32 + 24i
  \]
  so
  \[
  \lvert z_1\rvert = \sqrt{32^2 + 24^2} = 40.
  \]
  For the second problem, we have that
  \[
  z_2 = \frac{(3 + 4i)(-1 + 2i)}{(-1 - i)(3 - i)} = 2 - \frac{3}{2}i
  \]
  so
  \[
  \lvert z_2\rvert = \sqrt{4 + 9/4} = \frac{5}{2}.
  \]
\item
  Prove that
  \[
  \Bigl\lvert\frac{a - b}{1 - \bar{a}b}\Bigr\rvert = 1
  \]
  if either \(\lvert a\rvert = 1\) or \(\lvert b\rvert = 1\).
  What exception must be made if \(\lvert a\rvert = \lvert b\rvert = 1\)?
  \par\smallskip
  Recall that \(\lvert z\rvert^2 = z\bar{z}\).
  \begin{align*}
    1^2 & = \Bigl\lvert\frac{a - b}{1 - \bar{a}b}\Bigr\rvert^2\\
    1 & = \Bigl(\frac{a - b}{1 - \bar{a}b}\Bigr)
    \Bigl(\frac{\overline{a - b}}{\overline{1 - \bar{a}b}}\Bigr)\\
        & = \Bigl(\frac{a - b}{1 - \bar{a}b}\Bigr)
          \Bigl(\frac{\bar{a} - \bar{b}}{1 - a\bar{b}}\Bigr)\\
        & = \frac{a\bar{a} - a\bar{b} - \bar{a}b + b\bar{b}}
          {1 - \bar{a}b - a\bar{b} + a\bar{a}b\bar{b}}\eqnumtag\label{1.4.3}
  \end{align*}
  If \(\lvert a\rvert = 1\), then \(\lvert a\rvert^2 = a\bar{a} = 1\) and
  similarly for \(\lvert b\rvert^2 = 1\).
  Then \cref{1.4.3} becomes
  \[
  \frac{1 - a\bar{b} - \bar{a}b + b\bar{b}}{1 - \bar{a}b - a\bar{b} + b\bar{b}}
  \qquad\text{and}\qquad
  \frac{1 - a\bar{b} - \bar{a}b + a\bar{a}}{1 - \bar{a}b - a\bar{b} + a\bar{a}}
  \]
  resepctively which is one.
  If \(\lvert a\rvert = \lvert b\rvert = 1\), then
  \(\lvert a\rvert^2 = \vert b\rvert^2 = 1\) so \cref{1.4.3} can be written as
  \[
  \frac{2 - a\bar{b} - \bar{a}b}{2 - \bar{a}b - a\bar{b}}.
  \]
  Therefore, we must have that \(a\bar{b} + \bar{a}b\neq 2\).
\item
  Find the conditions under which the equation \(az + b\bar{z} + c = 0\) in one
  complex unknown has exactly one solution, and compute that solution.
  \par\smallskip
  Let \(z = x + iy\).
  Then \(az + b\bar{z} + c = a(x + iy) + b(x - iy) + c = 0\).
  \begin{subequations}
    \begin{align}
      (a + b)x + c & = 0\label{1.4.4R}\\
      (a - b)y & = 0\label{1.4.4I}
    \end{align}
  \end{subequations}
  Lets consider \cref{1.4.4I}.
  We either have that \(a = b\) or \(y = 0\).
  If \(a = b\), then WLOG \cref{1.4.4R} can be written as
  \[
  x = \frac{-c}{2a}
  \]
  and \(y\in\mathbb{R}\).
  For fixed \(a,b,c\), we have infinitely many solutions when \(a = b\) since
  \(z = \frac{-c}{2a} + iy\) for \(y\in\mathbb{R}\).
  If \(y = 0\), then \cref{1.4.4R} can be written as
  \[
  x = \frac{-c}{a + b}.
  \]
  Therefore, \(z = x\) and we have only one solution.
\item
  Prove that Lagrange's identity in the complex form
  \[
  \Bigl\lvert\sum_{i = 1}^na_ib_i\Bigr\rvert^2 =
  \sum_{i = 1}^n\lvert a_i\rvert^2\sum_{i = 1}^n\lvert b_i\rvert^2 -
  \smashoperator{\sum_{1\leq i\leq j\leq n}}
  \lvert a_i\bar{b}_j - a_j\bar{b}_i\rvert^2.
  \]
\end{enumerate}

\subsection{Inequalities}

%%% Local Variables:
%%% mode: latex
%%% TeX-master: t
%%% End:
